theories/Inference.v
@@ -1,2 +1,0 @@
-Require Import Checker.Variable.
-Require Import Checker.Atomic.
